fstar/MLS.TreeSync.API.Types.fst
@@ -14,7 +14,6 @@ type treesync_state (bytes:Type0) {|crypto_bytes bytes|} (tkt:treekem_types byte
   levels: nat;
   tree: treesync_valid bytes tkt levels 0 group_id;
   tokens: tokens:Ghost.erased (as_tokens bytes asp levels 0){all_credentials_ok tree tokens};
-  version: nat;
 }
 
 type treesync_index (#bytes:Type0) {|crypto_bytes bytes|} (#tkt:treekem_types bytes) (#asp:as_parameters bytes) (st:treesync_state bytes tkt asp) = i:nat{i < pow2 st.levels}
